Add basic x86 equiv checking, add x86 tutorials (#181)

x86/tutorial/simple.ml
@@ -10,25 +10,25 @@
 (* Please copy this file to the root directory of s2n-bignum, then
    follow the instructions. *)
 
-needs "arm/proofs/base.ml";;
+needs "x86/proofs/base.ml";;
 
 (* Let's prove a simple property of the following program:
 
-   0:   8b000022        add     x2, x1, x0
-   4:   cb010042        sub     x2, x2, x1
+    0:   48 01 c3                add    %rax,%rbx
+    3:   48 29 c3                sub    %rax,%rbx
 
   Let's start with defining a byte sequence of a program 'simple.S'
 *)
 let simple_mc = new_definition `simple_mc = [
-    word 0x22; word 0x00; word 0x00; word 0x8b; // add x2, x1, x0
-    word 0x42; word 0x00; word 0x01; word 0xcb  // sub x2, x2, x1
+    word 0x48; word 0x01; word 0xc3;
+    word 0x48; word 0x29; word 0xc3
   ]:((8)word)list`;;
 
 (* Or, you can read .o file and store the byte list as follows:
-let simple_mc = define_assert_from_elf "simple_mc" "arm/tutorial/simple.o"
+let simple_mc = define_assert_from_elf "simple_mc" "x86/tutorial/simple.o"
 [
-  0x8b000022;       (* arm_ADD X2 X1 X0 *)
-  0xcb010042        (* arm_SUB X2 X2 X1 *)
+  0x48; 0x01; 0xc3;        (* ADD (% rbx) (% rax) *)
+  0x48; 0x29; 0xc3         (* SUB (% rbx) (% rax) *)
 ];;
 
 You can get the above OCaml list data structure from
@@ -36,9 +36,9 @@ You can get the above OCaml list data structure from
 "<.o file>"`.
 *)
 
-(* ARM_MK_EXEC_RULE decodes the byte sequence into conjunction of
+(* X86_MK_EXEC_RULE decodes the byte sequence into conjunction of
   equalities between the bytes and instructions. *)
-let EXEC = ARM_MK_EXEC_RULE simple_mc;;
+let EXEC = X86_MK_EXEC_RULE simple_mc;;
 
 (*
   In s2n-bignum, a specification (ensures) has three components:
@@ -49,53 +49,55 @@ let EXEC = ARM_MK_EXEC_RULE simple_mc;;
   In this file,
   1. precondition is:
     - the 'simple' binary is loaded at some location in memory, say 'pc'
-    - the arm program counter register, PC, has value pc
-    - the arm register X0 has a symbolic value a and X1 has a symbolic value b
+    - the x86 program counter register, RIP, has value pc
+    - the x86 register RAX has a symbolic value a and RBX has a symbolic value b
   2. postcondition is:
-    - the arm program counter register, PC, has value pc+8
+    - the x86 program counter RIP, has value pc+6
       (meaning that two instructions have been executed)
-    - the arm register X2 has value b
+    - the x86 register RBX has value b
   3. frame is:
-    - the register values of PC and X2 might have been changed
+    - the register values of RIP, RBX and flags might have been changed
 
   If you are using the VSCode plugin of HOL Light, you can ctrl+click
   (cmd+click for Mac) to jump to definitions.
 *)
 let SIMPLE_SPEC = prove(
   `forall pc a b.
-  ensures arm
+  ensures x86
     // Precondition
-    (\s. // aligned_bytes_loaded states that a byte sequence 'simple_mc'
-         // is loaded at memory location 'pc' in the state 's' and also
-         // 4-bytes aligned.
-         aligned_bytes_loaded s (word pc) simple_mc /\
+    (\s. // bytes_loaded states that a byte sequence 'simple_mc'
+         // is loaded at memory location 'pc' in the state 's'.
+         bytes_loaded s (word pc) simple_mc /\
          // 'word' is a bit-vector type in HOL Light.
          // 'word a' means it is a bit-vector whose numeral (:num type)
          // is 'a'. Its bit-width is inferred as 64 bits here, but it can
          // be manually annotated as (word a:(64)word).
-         read PC s = word pc /\
-         read X0 s = word a /\
-         read X1 s = word b)
+         read RIP s = word pc /\
+         read RAX s = word a /\
+         read RBX s = word b)
     // Postcondition
-    (\s. read PC s = word (pc+8) /\
-         read X2 s = word a)
+    (\s. read RIP s = word (pc+6) /\
+         read RBX s = word b)
     // Registers (and memory locations) that may change after execution
-    (MAYCHANGE [PC;X2])`,
+    (MAYCHANGE [RIP;RBX] ,, MAYCHANGE SOME_FLAGS)`,
 
   (* Strips the outermost universal quantifier from the conclusion of a goal *)
   REPEAT STRIP_TAC THEN
+  (* ENSURES_FINAL_STATE_TAC does not understand SOME_FLAGS in MAYCHANGE. Let's
+     unfold this in advance. *)
+  REWRITE_TAC [SOME_FLAGS] THEN
   (* Start symbolic execution with state 's0' *)
   ENSURES_INIT_TAC "s0" THEN
 
   (* Symbolically run two instructions *)
-  ARM_STEPS_TAC EXEC (1--2) THEN
+  X86_STEPS_TAC EXEC (1--2) THEN
   (* Try to prove the postcondition and frame as much as possible *)
   ENSURES_FINAL_STATE_TAC THEN
 
   (* Use ASM_REWRITE_TAC[] to rewrite the goal using equalities in assumptions. *)
   ASM_REWRITE_TAC[] THEN
   (* We need to prove this:
-     `word_sub (word_add (word b) (word a)) (word b) = word a`
+     `word_sub (word_add (word b) (word a)) (word a) = word b`
      Use an automated prover for words in HOL Light *)
   CONV_TAC WORD_RULE);;
 
@@ -103,5 +105,5 @@ let SIMPLE_SPEC = prove(
    if its inputs do not have their symbolic expressions defined in assumption.
    To list which instructions are discarded by the simulation tactic.
    set:
-    arm_print_log := true;;
+    x86_print_log := true;;
    This flag will also print helpful informations that are useful. *)
